src/code/kubernetes_model/apimodel.v
@@ -2285,15 +2285,16 @@ Definition shouldDeleteDependentsⁱᵐᵖˡ : val :=
         else do:  #()))));;;
     return: (#false)).
 
+Definition deletionFinalizersForGarbageCollection : go_string := "kubernetes_model/apimodel.deletionFinalizersForGarbageCollection"%go.
+
 (* deletionFinalizersForGarbageCollection determines which finalizers should be set for garbage collection.
    It returns whether the finalizer list needs updating and the new finalizer list.
    Reference: https://github.com/kubernetes/kubernetes/blob/release-1.34/staging/src/k8s.io/apiserver/pkg/registry/generic/registry/store.go#L976-L1005
 
-   go: new.go:715:17 *)
-Definition State__deletionFinalizersForGarbageCollectionⁱᵐᵖˡ : val :=
-  λ: "s" "metadata" "options",
-    exception_do (let: "s" := (mem.alloc "s") in
-    let: "options" := (mem.alloc "options") in
+   go: new.go:715:6 *)
+Definition deletionFinalizersForGarbageCollectionⁱᵐᵖˡ : val :=
+  λ: "metadata" "options",
+    exception_do (let: "options" := (mem.alloc "options") in
     let: "metadata" := (mem.alloc "metadata") in
     let: "shouldOrphan" := (mem.alloc (type.zero_val #boolT)) in
     let: "$r0" := (let: "$a0" := (![#v1.Object] "metadata") in
@@ -2371,7 +2372,7 @@ Definition validateDeletePreconditions : go_string := "kubernetes_model/apimodel
    Returns a Conflict error if preconditions don't match.
    Reference: https://github.com/kubernetes/kubernetes/blob/release-1.34/staging/src/k8s.io/apiserver/pkg/registry/rest/delete.go (BeforeDelete)
 
-   go: new.go:765:6 *)
+   go: new.go:762:6 *)
 Definition validateDeletePreconditionsⁱᵐᵖˡ : val :=
   λ: "metadata" "options" "kind",
     exception_do (let: "kind" := (mem.alloc "kind") in
@@ -2424,7 +2425,7 @@ Definition checkGracefulDelete : go_string := "kubernetes_model/apimodel.checkGr
    Returns (graceful, pendingGraceful, error).
    Reference: https://github.com/kubernetes/kubernetes/blob/release-1.34/pkg/registry/core/pod/strategy.go#L162-L191
 
-   go: new.go:798:6 *)
+   go: new.go:795:6 *)
 Definition checkGracefulDeleteⁱᵐᵖˡ : val :=
   λ: "obj" "options",
     exception_do (let: "options" := (mem.alloc "options") in
@@ -2493,7 +2494,7 @@ Definition checkGracefulDeleteⁱᵐᵖˡ : val :=
          slice.literal #interfaceT ["$sl0"])) in
          (func_call #fmt.Errorf) "$a0" "$a1")))).
 
-(* go: new.go:837:17 *)
+(* go: new.go:834:17 *)
 Definition State__deleteⁱᵐᵖˡ : val :=
   λ: "s" "key" "options",
     with_defer: (let: "s" := (mem.alloc "s") in
@@ -2569,7 +2570,7 @@ Definition State__deleteⁱᵐᵖˡ : val :=
     let: "shouldUpdateFinalizers" := (mem.alloc (type.zero_val #boolT)) in
     let: ("$ret0", "$ret1") := (let: "$a0" := (![#v1.Object] "metadata") in
     let: "$a1" := "options" in
-    (method_call #(ptrT.id State.id) #"deletionFinalizersForGarbageCollection"%go (![#ptrT] "s")) "$a0" "$a1") in
+    (func_call #deletionFinalizersForGarbageCollection) "$a0" "$a1") in
     let: "$r0" := "$ret0" in
     let: "$r1" := "$ret1" in
     do:  ("shouldUpdateFinalizers" <-[#boolT] "$r0");;;
@@ -2639,7 +2640,7 @@ Definition State__deleteⁱᵐᵖˡ : val :=
    graceful deletion, and finalizer handling. Returns the deleted (or updated) Pod object.
    PodCreate2 creates a Pod using create, which includes admission controller logic.
 
-   go: new.go:928:17 *)
+   go: new.go:925:17 *)
 Definition State__PodCreate2ⁱᵐᵖˡ : val :=
   λ: "s" "namespace" "pod",
     exception_do (let: "s" := (mem.alloc "s") in
@@ -2676,7 +2677,7 @@ Definition State__PodCreate2ⁱᵐᵖˡ : val :=
 
 (* ReplicaSetCreate2 creates a ReplicaSet using create, which includes admission controller logic.
 
-   go: new.go:943:17 *)
+   go: new.go:940:17 *)
 Definition State__ReplicaSetCreate2ⁱᵐᵖˡ : val :=
   λ: "s" "namespace" "rs",
     exception_do (let: "s" := (mem.alloc "s") in
@@ -2713,7 +2714,7 @@ Definition State__ReplicaSetCreate2ⁱᵐᵖˡ : val :=
 
 (* PodUpdate2 updates a Pod using the richer storage/update model.
 
-   go: new.go:958:17 *)
+   go: new.go:955:17 *)
 Definition State__PodUpdate2ⁱᵐᵖˡ : val :=
   λ: "s" "namespace" "pod",
     exception_do (let: "s" := (mem.alloc "s") in
@@ -2750,7 +2751,7 @@ Definition State__PodUpdate2ⁱᵐᵖˡ : val :=
 
 (* ReplicaSetUpdate2 updates a ReplicaSet using the richer storage/update model.
 
-   go: new.go:973:17 *)
+   go: new.go:970:17 *)
 Definition State__ReplicaSetUpdate2ⁱᵐᵖˡ : val :=
   λ: "s" "namespace" "rs",
     exception_do (let: "s" := (mem.alloc "s") in
@@ -2787,7 +2788,7 @@ Definition State__ReplicaSetUpdate2ⁱᵐᵖˡ : val :=
 
 (* PodDelete2 deletes a Pod with full DeleteOptions support, including graceful deletion.
 
-   go: new.go:988:17 *)
+   go: new.go:985:17 *)
 Definition State__PodDelete2ⁱᵐᵖˡ : val :=
   λ: "s" "namespace" "name" "options",
     exception_do (let: "s" := (mem.alloc "s") in
@@ -2811,7 +2812,7 @@ Definition State__PodDelete2ⁱᵐᵖˡ : val :=
 (* ReplicaSetDelete2 deletes a ReplicaSet with full DeleteOptions support.
    ReplicaSets don't support graceful deletion but do support finalizers and preconditions.
 
-   go: new.go:995:17 *)
+   go: new.go:992:17 *)
 Definition State__ReplicaSetDelete2ⁱᵐᵖˡ : val :=
   λ: "s" "namespace" "name" "options",
     exception_do (let: "s" := (mem.alloc "s") in
@@ -2834,9 +2835,9 @@ Definition State__ReplicaSetDelete2ⁱᵐᵖˡ : val :=
 
 Definition vars' : list (go_string * go_type) := [].
 
-Definition functions' : list (go_string * val) := [(NewState, NewStateⁱᵐᵖˡ); (deepCopy, deepCopyⁱᵐᵖˡ); (filterByLabelSelector, filterByLabelSelectorⁱᵐᵖˡ); (index_of, index_ofⁱᵐᵖˡ); (randomSuffix, randomSuffixⁱᵐᵖˡ); (validateObjectMeta, validateObjectMetaⁱᵐᵖˡ); (applyDefaultTolerationSeconds, applyDefaultTolerationSecondsⁱᵐᵖˡ); (applyPriorityAdmission, applyPriorityAdmissionⁱᵐᵖˡ); (convertVersionedToLegacy, convertVersionedToLegacyⁱᵐᵖˡ); (applySchemaDefaults, applySchemaDefaultsⁱᵐᵖˡ); (applyStrategyPrepareForCreate, applyStrategyPrepareForCreateⁱᵐᵖˡ); (applyAdmissionMutate, applyAdmissionMutateⁱᵐᵖˡ); (applyAdmissionMutateForUpdate, applyAdmissionMutateForUpdateⁱᵐᵖˡ); (applyAdmissionValidate, applyAdmissionValidateⁱᵐᵖˡ); (allowUnconditionalUpdate, allowUnconditionalUpdateⁱᵐᵖˡ); (malformedUpdateResourceVersionError, malformedUpdateResourceVersionErrorⁱᵐᵖˡ); (updateStrategyForLegacyObject, updateStrategyForLegacyObjectⁱᵐᵖˡ); (applyStrategyValidate, applyStrategyValidateⁱᵐᵖˡ); (applyStrategyCanonicalize, applyStrategyCanonicalizeⁱᵐᵖˡ); (applyValidationAndDefaultingOnUpdate, applyValidationAndDefaultingOnUpdateⁱᵐᵖˡ); (applyValidationAndDefaulting, applyValidationAndDefaultingⁱᵐᵖˡ); (shouldOrphanDependents, shouldOrphanDependentsⁱᵐᵖˡ); (shouldDeleteDependents, shouldDeleteDependentsⁱᵐᵖˡ); (validateDeletePreconditions, validateDeletePreconditionsⁱᵐᵖˡ); (checkGracefulDelete, checkGracefulDeleteⁱᵐᵖˡ)].
+Definition functions' : list (go_string * val) := [(NewState, NewStateⁱᵐᵖˡ); (deepCopy, deepCopyⁱᵐᵖˡ); (filterByLabelSelector, filterByLabelSelectorⁱᵐᵖˡ); (index_of, index_ofⁱᵐᵖˡ); (randomSuffix, randomSuffixⁱᵐᵖˡ); (validateObjectMeta, validateObjectMetaⁱᵐᵖˡ); (applyDefaultTolerationSeconds, applyDefaultTolerationSecondsⁱᵐᵖˡ); (applyPriorityAdmission, applyPriorityAdmissionⁱᵐᵖˡ); (convertVersionedToLegacy, convertVersionedToLegacyⁱᵐᵖˡ); (applySchemaDefaults, applySchemaDefaultsⁱᵐᵖˡ); (applyStrategyPrepareForCreate, applyStrategyPrepareForCreateⁱᵐᵖˡ); (applyAdmissionMutate, applyAdmissionMutateⁱᵐᵖˡ); (applyAdmissionMutateForUpdate, applyAdmissionMutateForUpdateⁱᵐᵖˡ); (applyAdmissionValidate, applyAdmissionValidateⁱᵐᵖˡ); (allowUnconditionalUpdate, allowUnconditionalUpdateⁱᵐᵖˡ); (malformedUpdateResourceVersionError, malformedUpdateResourceVersionErrorⁱᵐᵖˡ); (updateStrategyForLegacyObject, updateStrategyForLegacyObjectⁱᵐᵖˡ); (applyStrategyValidate, applyStrategyValidateⁱᵐᵖˡ); (applyStrategyCanonicalize, applyStrategyCanonicalizeⁱᵐᵖˡ); (applyValidationAndDefaultingOnUpdate, applyValidationAndDefaultingOnUpdateⁱᵐᵖˡ); (applyValidationAndDefaulting, applyValidationAndDefaultingⁱᵐᵖˡ); (shouldOrphanDependents, shouldOrphanDependentsⁱᵐᵖˡ); (shouldDeleteDependents, shouldDeleteDependentsⁱᵐᵖˡ); (deletionFinalizersForGarbageCollection, deletionFinalizersForGarbageCollectionⁱᵐᵖˡ); (validateDeletePreconditions, validateDeletePreconditionsⁱᵐᵖˡ); (checkGracefulDelete, checkGracefulDeleteⁱᵐᵖˡ)].
 
-Definition msets' : list (go_string * (list (go_string * val))) := [(State.id, []); (ptrT.id State.id, [("ByIndex"%go, State__ByIndexⁱᵐᵖˡ); ("Index"%go, State__Indexⁱᵐᵖˡ); ("PodCreate"%go, State__PodCreateⁱᵐᵖˡ); ("PodCreate2"%go, State__PodCreate2ⁱᵐᵖˡ); ("PodDelete"%go, State__PodDeleteⁱᵐᵖˡ); ("PodDelete2"%go, State__PodDelete2ⁱᵐᵖˡ); ("PodGet"%go, State__PodGetⁱᵐᵖˡ); ("PodList"%go, State__PodListⁱᵐᵖˡ); ("PodMutGet"%go, State__PodMutGetⁱᵐᵖˡ); ("PodMutList"%go, State__PodMutListⁱᵐᵖˡ); ("PodUpdate"%go, State__PodUpdateⁱᵐᵖˡ); ("PodUpdate2"%go, State__PodUpdate2ⁱᵐᵖˡ); ("ReplicaSetCreate2"%go, State__ReplicaSetCreate2ⁱᵐᵖˡ); ("ReplicaSetDelete2"%go, State__ReplicaSetDelete2ⁱᵐᵖˡ); ("ReplicaSetGet"%go, State__ReplicaSetGetⁱᵐᵖˡ); ("ReplicaSetMutGet"%go, State__ReplicaSetMutGetⁱᵐᵖˡ); ("ReplicaSetUpdate2"%go, State__ReplicaSetUpdate2ⁱᵐᵖˡ); ("create"%go, State__createⁱᵐᵖˡ); ("delete"%go, State__deleteⁱᵐᵖˡ); ("deletionFinalizersForGarbageCollection"%go, State__deletionFinalizersForGarbageCollectionⁱᵐᵖˡ); ("generateNewName"%go, State__generateNewNameⁱᵐᵖˡ); ("generateNewRVAndUpdate"%go, State__generateNewRVAndUpdateⁱᵐᵖˡ); ("generateNewUIDAndUpdate"%go, State__generateNewUIDAndUpdateⁱᵐᵖˡ); ("get"%go, State__getⁱᵐᵖˡ); ("objCreate"%go, State__objCreateⁱᵐᵖˡ); ("objDelete"%go, State__objDeleteⁱᵐᵖˡ); ("objGet"%go, State__objGetⁱᵐᵖˡ); ("objList"%go, State__objListⁱᵐᵖˡ); ("objListBySelector"%go, State__objListBySelectorⁱᵐᵖˡ); ("objListLocked"%go, State__objListLockedⁱᵐᵖˡ); ("objUpdate"%go, State__objUpdateⁱᵐᵖˡ); ("update"%go, State__updateⁱᵐᵖˡ)]); (KKey.id, []); (ptrT.id KKey.id, [])].
+Definition msets' : list (go_string * (list (go_string * val))) := [(State.id, []); (ptrT.id State.id, [("ByIndex"%go, State__ByIndexⁱᵐᵖˡ); ("Index"%go, State__Indexⁱᵐᵖˡ); ("PodCreate"%go, State__PodCreateⁱᵐᵖˡ); ("PodCreate2"%go, State__PodCreate2ⁱᵐᵖˡ); ("PodDelete"%go, State__PodDeleteⁱᵐᵖˡ); ("PodDelete2"%go, State__PodDelete2ⁱᵐᵖˡ); ("PodGet"%go, State__PodGetⁱᵐᵖˡ); ("PodList"%go, State__PodListⁱᵐᵖˡ); ("PodMutGet"%go, State__PodMutGetⁱᵐᵖˡ); ("PodMutList"%go, State__PodMutListⁱᵐᵖˡ); ("PodUpdate"%go, State__PodUpdateⁱᵐᵖˡ); ("PodUpdate2"%go, State__PodUpdate2ⁱᵐᵖˡ); ("ReplicaSetCreate2"%go, State__ReplicaSetCreate2ⁱᵐᵖˡ); ("ReplicaSetDelete2"%go, State__ReplicaSetDelete2ⁱᵐᵖˡ); ("ReplicaSetGet"%go, State__ReplicaSetGetⁱᵐᵖˡ); ("ReplicaSetMutGet"%go, State__ReplicaSetMutGetⁱᵐᵖˡ); ("ReplicaSetUpdate2"%go, State__ReplicaSetUpdate2ⁱᵐᵖˡ); ("create"%go, State__createⁱᵐᵖˡ); ("delete"%go, State__deleteⁱᵐᵖˡ); ("generateNewName"%go, State__generateNewNameⁱᵐᵖˡ); ("generateNewRVAndUpdate"%go, State__generateNewRVAndUpdateⁱᵐᵖˡ); ("generateNewUIDAndUpdate"%go, State__generateNewUIDAndUpdateⁱᵐᵖˡ); ("get"%go, State__getⁱᵐᵖˡ); ("objCreate"%go, State__objCreateⁱᵐᵖˡ); ("objDelete"%go, State__objDeleteⁱᵐᵖˡ); ("objGet"%go, State__objGetⁱᵐᵖˡ); ("objList"%go, State__objListⁱᵐᵖˡ); ("objListBySelector"%go, State__objListBySelectorⁱᵐᵖˡ); ("objListLocked"%go, State__objListLockedⁱᵐᵖˡ); ("objUpdate"%go, State__objUpdateⁱᵐᵖˡ); ("update"%go, State__updateⁱᵐᵖˡ)]); (KKey.id, []); (ptrT.id KKey.id, [])].
 
 #[global] Instance info' : PkgInfo apimodel.apimodel :=
   {|
