src/proof/pure_objects.v
@@ -211,6 +211,7 @@ Definition deepown (c: v1.ObjectMeta.t) (v: t) dq: iProp Σ :=
   "%Hdeepown_resourceversion" ∷ ⌜ c.(v1.ObjectMeta.ResourceVersion') = v.(ResourceVersion') ⌝ ∗
   "%Hdeepown_generation" ∷ ⌜ c.(v1.ObjectMeta.Generation') = v.(Generation') ⌝ ∗
   "Hdeepown_creationtimestamp" ∷ TimeV.deepown c.(v1.ObjectMeta.CreationTimestamp') v.(CreationTimestamp') ∗
+  (* TODO: define this repeated pattern to reduce the code below *)
   "%Hdeepown_deletiontimestamp_none" ∷ ⌜c.(v1.ObjectMeta.DeletionTimestamp') = null ↔ v.(DeletionTimestamp') = None⌝ ∗
   "Hdeepown_deletiontimestamp_some" ∷ (match v.(DeletionTimestamp') with
   | Some vd => ∃ cd, c.(v1.ObjectMeta.DeletionTimestamp') ↦{dq} cd ∗ TimeV.deepown cd vd
